Caso SEQ compilatore LOOP -> SCORE. Modificato nome funzione compilazione

MasterThesis/SCORE/Compiler.lean
@@ -7,33 +7,33 @@ namespace SCORE
 
 open SCORE.com
 
-def LOOP2SCORE (Lc : LOOP.com) : SCORE.com :=
+def L2S (Lc : LOOP.com) : SCORE.com :=
   match Lc with
   | LOOP.com.SKIP    => SKIP
   | LOOP.com.ZER x   => CON x
   | LOOP.com.ASN x y => CON x ;;
                         FOR y (INC x)
   | LOOP.com.INC x   => INC x
-  | LOOP.com.SEQ P Q => LOOP2SCORE P ;;
-                        LOOP2SCORE Q
+  | LOOP.com.SEQ P Q => L2S P ;;
+                        L2S Q
 
-  | LOOP.com.FOR x P => FOR x (LOOP2SCORE P)
+  | LOOP.com.FOR x P => FOR x (L2S P)
 
-namespace LOOP2SCORE
+namespace L2S
 
 def eqStores (σ : LOOP.store) (τ : SCORE.store) : Prop :=
   ∀ (x : ident), σ x = List.head! (τ x)
 
 infix:100 "=ₛ" => eqStores
 
-theorem soundness (LP : LOOP.com) (σ : LOOP.store) (τ : SCORE.store) : σ =ₛ τ → (LOOP.eval LP σ) =ₛ (SCORE.eval (LOOP2SCORE LP) τ) := by
+theorem soundness (LP : LOOP.com) (σ : LOOP.store) (τ : SCORE.store) : σ =ₛ τ → (LOOP.eval LP σ) =ₛ (SCORE.eval (L2S LP) τ) := by
   intros
-  induction LP with
+  induction LP generalizing σ τ with
   | SKIP =>
-    simp[LOOP.eval, LOOP2SCORE, SCORE.eval]
+    simp[LOOP.eval, L2S, SCORE.eval]
     assumption
   | ZER x =>
-    simp[LOOP.eval, LOOP2SCORE, SCORE.eval]
+    simp[LOOP.eval, L2S, SCORE.eval]
     intro y
     cases eq_or_ne x y with
     | inl =>
@@ -43,7 +43,7 @@ theorem soundness (LP : LOOP.com) (σ : LOOP.store) (τ : SCORE.store) : σ =ₛ
       apply ‹σ =ₛ τ› y
   | ASN x y => sorry
   | INC x =>
-    simp[LOOP.eval, LOOP2SCORE, SCORE.eval]
+    simp[LOOP.eval, L2S, SCORE.eval]
     intro y
     cases eq_or_ne x y with
     | inl =>
@@ -52,9 +52,11 @@ theorem soundness (LP : LOOP.com) (σ : LOOP.store) (τ : SCORE.store) : σ =ₛ
     | inr =>
       simp[List.head!, store.update_other ‹x ≠ y›, LOOP.store.update_other ‹x ≠ y›]
       apply ‹σ =ₛ τ› y
-  | SEQ LQ LR => sorry
+  | SEQ LQ LR ih₁ ih₂ =>
+     simp[LOOP.eval, L2S, SCORE.eval]
+     apply ih₂ (LOOP.eval LQ σ) (eval (L2S LQ) τ) (ih₁ σ τ ‹σ =ₛ τ›)
   | FOR x LQ => sorry
 
-end LOOP2SCORE
+end L2S
 
 end SCORE
